theories/iris/logrel/fundamental.v
@@ -38,13 +38,13 @@ Section Fundamental.
   Lemma compat_nop M F L wl wl' es' :
     let me := me_of_context M mr in
     let fe := fe_of_context F in
-    local_ctx_ok F L ->
     let ψ := InstrT [] [] in
+    has_instruction_type_ok F ψ L ->
     run_codegen (compile_instr me fe (INop ψ)) wl = inr ((), wl', es') ->
     ⊢ have_instruction_type_sem sr mr M F L [] (to_e_list es') ψ L.
   Proof.
     (* This is currently following the compat_copy lemma very closely *)
-    intros me fe HL ψ Hcompile.
+    intros me fe ψ Hok Hcompile.
     inv_cg_emit Hcompile.
     unfold have_instruction_type_sem.
     destruct ψ eqn:Hψ.
@@ -131,14 +131,13 @@ Section Fundamental.
   Lemma compat_copy M F L wl wl' τ es' :
     let me := me_of_context M mr in
     let fe := fe_of_context F in
-    local_ctx_ok F L ->
-    has_copyability F τ ExCopy ->
-    has_mono_rep F τ ->
     let ψ := InstrT [τ] [τ; τ] in
+    has_copyability F τ ExCopy ->
+    has_instruction_type_ok F ψ L ->
     run_codegen (compile_instr me fe (ICopy ψ)) wl = inr ((), wl', es') ->
     ⊢ have_instruction_type_sem sr mr M F L [] (to_e_list es') ψ L.
   Proof.
-    intros me fe HL Hcopy Hmono ψ Hcompile.
+    intros me fe ψ Hcopy Hok Hcompile.
     unfold compile_instr in Hcompile.
     cbn in Hcompile.
     inv_cg_bind Hcompile ρ wl1 es_nil es1 Htype_rep Hcompile.
@@ -173,7 +172,8 @@ Section Fundamental.
     rewrite big_sepL2_singleton.
     iApply (lwp_wand with "[Hframe]"); last first.
     - iApply ("Hcopyable" with "[] [] [$Hfr] [$Hrun] [$Hvs]").
-      + rewrite subst_repr_closed_nop; [|eapply mono_rep_closed; eauto; econstructor; eauto].
+      + inversion Hok. inversion H. inversion H4.
+        rewrite subst_repr_closed_nop; [|eapply mono_rep_closed; eauto; econstructor; eauto].
         iPureIntro. exact Heq_some0.
       + iPureIntro. unfold is_copy_operation. repeat eexists. apply Hcompile.
     - iIntros (lv) "(Hcopy & %fr' & Hfr & <-)".
@@ -194,10 +194,9 @@ Section Fundamental.
   Lemma compat_drop M F L wl wl' τ es' :
     let me := me_of_context M mr in
     let fe := fe_of_context F in
-    local_ctx_ok F L ->
-    has_dropability F τ ExDrop ->
-    has_mono_rep F τ ->
     let ψ := InstrT [τ] [] in
+    has_dropability F τ ExDrop ->
+    has_instruction_type_ok F ψ L ->
     run_codegen (compile_instr me fe (IDrop ψ)) wl = inr ((), wl', es') ->
     ⊢ have_instruction_type_sem sr mr M F L [] (to_e_list es') ψ L.
   Admitted.
@@ -205,8 +204,8 @@ Section Fundamental.
   Lemma compat_num M F L wl wl' ψ e es' :
     let me := me_of_context M mr in
     let fe := fe_of_context F in
-    local_ctx_ok F L ->
     has_instruction_type_num e ψ ->
+    has_instruction_type_ok F ψ L ->
     run_codegen (compile_instr me fe (INum ψ e)) wl = inr ((), wl', es') ->
     ⊢ have_instruction_type_sem sr mr M F L [] (to_e_list es') ψ L.
   Admitted.
@@ -214,9 +213,8 @@ Section Fundamental.
   Lemma compat_num_const M F L wl wl' n ν κ es' :
     let me := me_of_context M mr in
     let fe := fe_of_context F in
-    local_ctx_ok F L ->
-    has_kind F (NumT κ ν) κ ->
     let ψ := InstrT [] [NumT κ ν] in
+    has_instruction_type_ok F ψ L ->
     run_codegen (compile_instr me fe (INumConst ψ n)) wl = inr ((), wl', es') ->
     ⊢ have_instruction_type_sem sr mr M F L [] (to_e_list es') ψ L.
   Admitted.
@@ -226,6 +224,7 @@ Section Fundamental.
     let fe := fe_of_context F in
     let F' := F <| fc_labels ::= cons (τs2, L') |> in
     let ψ := InstrT τs1 τs2 in
+    has_instruction_type_ok F ψ L' ->
     (forall wl wl' es',
         let fe' := fe_of_context F' in
         run_codegen (compile_instrs me fe' es) wl = inr ((), wl', es') ->
@@ -239,6 +238,7 @@ Section Fundamental.
     let fe := fe_of_context F in
     let F' := F <| fc_labels ::= cons (τs1, L) |> in
     let ψ := InstrT τs1 τs2 in
+    has_instruction_type_ok F ψ L ->
     (forall wl wl' es',
         let fe' := fe_of_context F' in
         run_codegen (compile_instrs me fe' es) wl = inr ((), wl', es') ->
@@ -251,12 +251,13 @@ Section Fundamental.
     let me := me_of_context M mr in
     let fe := fe_of_context F in
     let ψ := InstrT (τs1 ++ [type_i32]) τs2 in
+    has_instruction_type_ok F ψ L' ->
     (forall wl wl' es',
         run_codegen (compile_instrs me fe es1) wl = inr ((), wl', es') ->
         ⊢ have_instruction_type_sem sr mr M F L wl' (to_e_list es') (InstrT τs1 τs2) L') ->
     (forall wl wl' es',
-        run_codegen (compile_instrs me fe es2) wl = inr ((), wl', es')
-        → ⊢ have_instruction_type_sem sr mr M F L wl' (to_e_list es') (InstrT τs1 τs2) L') ->
+        run_codegen (compile_instrs me fe es2) wl = inr ((), wl', es') ->
+        ⊢ have_instruction_type_sem sr mr M F L wl' (to_e_list es') (InstrT τs1 τs2) L') ->
     run_codegen (compile_instr me fe (IIte ψ L' es1 es2)) wl = inr ((), wl', es') ->
     ⊢ have_instruction_type_sem sr mr M F L [] (to_e_list es') ψ L'.
   Admitted.
@@ -264,9 +265,9 @@ Section Fundamental.
   Lemma compat_br M F L L' wl wl' es' i τs1 τs τs2 :
     let me := me_of_context M mr in
     let fe := fe_of_context F in
+    let ψ := InstrT (τs1 ++ τs) τs2 in
     F.(fc_labels) !! i = Some (τs, L) ->
     Forall (fun τ => has_dropability F τ ImDrop) τs1 ->
-    let ψ := InstrT (τs1 ++ τs) τs2 in
     has_instruction_type_ok F ψ L' ->
     run_codegen (compile_instr me fe (IBr ψ i)) wl = inr ((), wl', es') ->
     ⊢ have_instruction_type_sem sr mr M F L [] (to_e_list es') ψ L'.
@@ -275,9 +276,9 @@ Section Fundamental.
   Lemma compat_return M F L L' wl wl' es' τs1 τs τs2 :
     let me := me_of_context M mr in
     let fe := fe_of_context F in
+    let ψ := InstrT (τs1 ++ τs) τs2 in
     F.(fc_return) = τs ->
     Forall (fun τ => has_dropability F τ ImDrop) τs1 ->
-    let ψ := InstrT (τs1 ++ τs) τs2 in
     has_instruction_type_ok F ψ L' ->
     run_codegen (compile_instr me fe (IReturn ψ)) wl = inr ((), wl', es') ->
     ⊢ have_instruction_type_sem sr mr M F L [] (to_e_list es') ψ L'.
@@ -286,85 +287,81 @@ Section Fundamental.
   Lemma compat_local_get M F L wl wl' es' i τ ιs :
     let me := me_of_context M mr in
     let fe := fe_of_context F in
-    local_ctx_ok F L ->
-    F.(typing.fc_locals) !! i = Some ιs ->
-    L !! i = Some τ ->
+    let ψ := InstrT [] [τ] in
     let ρ := ProdR (map PrimR ιs) in
     let τ' := RepT (VALTYPE ρ ImCopy ImDrop) ρ (ProdT (VALTYPE (ProdR []) ImCopy ImDrop) []) in
-    let L' := <[i:=τ']> L in
-    let ψ := InstrT [] [τ] in
+    let L' := <[ i := τ']> L in
+    F.(typing.fc_locals) !! i = Some ιs ->
+    L !! i = Some τ ->
+    has_instruction_type_ok F ψ L' ->
     run_codegen (compile_instr me fe (ILocalGet ψ i)) wl = inr ((), wl', es') ->
     ⊢ have_instruction_type_sem sr mr M F L [] (to_e_list es') ψ L'.
   Admitted.
 
-  Lemma compat_local_get_copy M F L wl wl' es' n τ :
+  Lemma compat_local_get_copy M F L wl wl' es' i τ :
     let me := me_of_context M mr in
     let fe := fe_of_context F in
-    local_ctx_ok F L ->
-    L !! n = Some τ ->
-    has_copyability F τ ImCopy ->
     let ψ := InstrT [] [τ] in
-    run_codegen (compile_instr me fe (ILocalGet ψ n)) wl = inr ((), wl', es') ->
+    L !! i = Some τ ->
+    has_copyability F τ ImCopy ->
+    has_instruction_type_ok F ψ L ->
+    run_codegen (compile_instr me fe (ILocalGet ψ i)) wl = inr ((), wl', es') ->
     ⊢ have_instruction_type_sem sr mr M F L [] (to_e_list es') ψ L.
   Admitted.
 
   Lemma compat_local_set M F L wl wl' es' i τ τ' ιs :
     let me := me_of_context M mr in
     let fe := fe_of_context F in
-    local_ctx_ok F L ->
-    F.(typing.fc_locals) !! i = Some ιs ->
+    let ψ := InstrT [τ'] [] in
+    let L' := <[ i := τ']> L in
     L !! i = Some τ ->
     has_dropability F τ ImDrop ->
+    F.(typing.fc_locals) !! i = Some ιs ->
     type_rep_eval F τ' ιs ->
-    let L' := <[ i := τ' ]> L in
-    let ψ := InstrT [τ'] [] in
+    has_instruction_type_ok F ψ L' ->
     run_codegen (compile_instr me fe (ILocalSet ψ i)) wl = inr ((), wl', es') ->
     ⊢ have_instruction_type_sem sr mr M F L [] (to_e_list es') ψ L'.
   Admitted.
 
-  Lemma compat_global_get M F L wl wl' es' n m τ :
+  Lemma compat_global_get M F L wl wl' es' i ω τ :
     let me := me_of_context M mr in
     let fe := fe_of_context F in
-    local_ctx_ok F L ->
-    mc_globals M !! n = Some (m, τ) ->
-    has_mono_rep F τ ->
-    has_copyability F τ ImCopy ->
     let ψ := InstrT [] [τ] in
-    run_codegen (compile_instr me fe (IGlobalGet ψ n)) wl = inr ((), wl', es') ->
+    M.(mc_globals) !! i = Some (ω, τ) ->
+    has_copyability F τ ImCopy ->
+    has_instruction_type_ok F ψ L ->
+    run_codegen (compile_instr me fe (IGlobalGet ψ i)) wl = inr ((), wl', es') ->
     ⊢ have_instruction_type_sem sr mr M F L [] (to_e_list es') ψ L.
   Admitted.
 
-  Lemma compat_global_set M F L wl wl' es' n τ :
+  Lemma compat_global_set M F L wl wl' es' i τ :
     let me := me_of_context M mr in
     let fe := fe_of_context F in
-    local_ctx_ok F L ->
-    mc_globals M !! n = Some (Mut, τ) ->
-    has_mono_rep F τ ->
-    has_dropability F τ ImDrop ->
     let ψ := InstrT [τ] [] in
-    run_codegen (compile_instr me fe (IGlobalSet ψ n)) wl = inr ((), wl', es') ->
+    M.(mc_globals) !! i = Some (Mut, τ) ->
+    has_dropability F τ ImDrop ->
+    has_instruction_type_ok F ψ L ->
+    run_codegen (compile_instr me fe (IGlobalSet ψ i)) wl = inr ((), wl', es') ->
     ⊢ have_instruction_type_sem sr mr M F L [] (to_e_list es') ψ L.
   Admitted.
 
-  Lemma compat_global_swap M F L wl wl' es' n τ :
+  Lemma compat_global_swap M F L wl wl' es' i τ :
     let me := me_of_context M mr in
     let fe := fe_of_context F in
-    local_ctx_ok F L ->
-    mc_globals M !! n = Some (Mut, τ) ->
-    has_mono_rep F τ ->
     let ψ := InstrT [τ] [τ] in
-    run_codegen (compile_instr me fe (IGlobalSwap ψ n)) wl = inr ((), wl', es') ->
+    M.(mc_globals) !! i = Some (Mut, τ) ->
+    has_instruction_type_ok F ψ L ->
+    run_codegen (compile_instr me fe (IGlobalSwap ψ i)) wl = inr ((), wl', es') ->
     ⊢ have_instruction_type_sem sr mr M F L [] (to_e_list es') ψ L.
   Admitted.
 
   Lemma compat_coderef M F L wl wl' es' i ϕ :
     let me := me_of_context M mr in
     let fe := fe_of_context F in
-    local_ctx_ok F L ->
-    mc_table M !! i = Some ϕ ->
-    function_type_ok F ϕ ->
     let τ := CodeRefT (VALTYPE (PrimR I32R) ImCopy ImDrop) ϕ in
     let ψ := InstrT [] [τ] in
+    M.(mc_table) !! i = Some ϕ ->
+    has_instruction_type_ok F ψ L ->
     run_codegen (compile_instr me fe (ICodeRef ψ i)) wl = inr ((), wl', es') ->
     ⊢ have_instruction_type_sem sr mr M F L [] (to_e_list es') ψ L.
   Admitted.
@@ -372,11 +369,10 @@ Section Fundamental.
   Lemma compat_inst M F L wl wl' es' ix ϕ ϕ' :
     let me := me_of_context M mr in
     let fe := fe_of_context F in
-    local_ctx_ok F L ->
-    function_type_ok F ϕ ->
-    function_type_inst F ix ϕ ϕ' ->
     let κ := VALTYPE (PrimR I32R) ImCopy ImDrop in
     let ψ := InstrT [CodeRefT κ ϕ] [CodeRefT κ ϕ'] in
+    function_type_inst F ix ϕ ϕ' ->
+    has_instruction_type_ok F ψ L ->
     run_codegen (compile_instr me fe (IInst ψ ix)) wl = inr ((), wl', es') ->
     ⊢ have_instruction_type_sem sr mr M F L [] (to_e_list es') ψ L.
   Admitted.
@@ -384,9 +380,9 @@ Section Fundamental.
   Lemma compat_call M F L wl wl' es' i ixs ϕ τs1 τs2 :
     let me := me_of_context M mr in
     let fe := fe_of_context F in
+    let ψ := InstrT τs1 τs2 in
     M.(mc_functions) !! i = Some ϕ ->
     function_type_insts F ixs ϕ (MonoFunT τs1 τs2) ->
-    let ψ := InstrT τs1 τs2 in
     has_instruction_type_ok F ψ L ->
     run_codegen (compile_instr me fe (ICall ψ i ixs)) wl = inr ((), wl', es') ->
     ⊢ have_instruction_type_sem sr mr M F L [] (to_e_list es') ψ L.
@@ -395,9 +391,9 @@ Section Fundamental.
   Lemma compat_call_indirect M F L wl wl' es' τs1 τs2 :
     let me := me_of_context M mr in
     let fe := fe_of_context F in
-    has_instruction_type_ok F (InstrT τs1 τs2) L ->
     let κ := VALTYPE (PrimR I32R) ImCopy ImDrop in
     let ψ := InstrT (τs1 ++ [CodeRefT κ (MonoFunT τs1 τs2)]) τs2 in
+    has_instruction_type_ok F ψ L ->
     run_codegen (compile_instr me fe (ICallIndirect ψ)) wl = inr ((), wl', es') ->
     ⊢ have_instruction_type_sem sr mr M F L [] (to_e_list es') ψ L.
   Admitted.
@@ -405,11 +401,9 @@ Section Fundamental.
   Lemma compat_inject M F L wl wl' es' i τs τ κ :
     let me := me_of_context M mr in
     let fe := fe_of_context F in
-    local_ctx_ok F L ->
-    τs !! i = Some τ ->
-    has_kind F (SumT κ τs) κ ->
-    Forall (has_mono_rep F) τs ->
     let ψ := InstrT [τ] [SumT κ τs] in
+    τs !! i = Some τ ->
+    has_instruction_type_ok F ψ L ->
     run_codegen (compile_instr me fe (IInject ψ i)) wl = inr ((), wl', es') ->
     ⊢ have_instruction_type_sem sr mr M F L [] (to_e_list es') ψ L.
   Admitted.
@@ -417,16 +411,14 @@ Section Fundamental.
   Lemma compat_case M F L L' wl wl' es' ess τs τ' κ :
     let me := me_of_context M mr in
     let fe := fe_of_context F in
-    local_ctx_ok F L' ->
-    has_mono_rep F τ' ->
-    Forall2
-      (fun τ es =>
-         (forall wl wl' es',
-             run_codegen (compile_instrs me fe es) wl = inr ((), wl', es') ->
-             ⊢ have_instruction_type_sem sr mr M F L wl' (to_e_list es') (InstrT [τ] [τ']) L'))
-      τs ess ->
-    has_kind F (SumT κ τs) κ ->
     let ψ := InstrT [SumT κ τs] [τ'] in
+    (Forall2
+      (fun τ es =>
+         forall wl wl' es',
+           run_codegen (compile_instrs me fe es) wl = inr ((), wl', es') ->
+           ⊢ have_instruction_type_sem sr mr M F L wl' (to_e_list es') (InstrT [τ] [τ']) L')
+      τs ess) ->
+    has_instruction_type_ok F ψ L' ->
     run_codegen (compile_instr me fe (ICase ψ L' ess)) wl = inr ((), wl', es') ->
     ⊢ have_instruction_type_sem sr mr M F L [] (to_e_list es') ψ L'.
   Admitted.
@@ -434,10 +426,8 @@ Section Fundamental.
   Lemma compat_group M F L wl wl' es' τs κ :
     let me := me_of_context M mr in
     let fe := fe_of_context F in
-    local_ctx_ok F L ->
-    Forall (has_mono_rep F) τs ->
-    has_kind F (ProdT κ τs) κ ->
     let ψ := InstrT τs [ProdT κ τs] in
+    has_instruction_type_ok F ψ L ->
     run_codegen (compile_instr me fe (IGroup ψ)) wl = inr ((), wl', es') ->
     ⊢ have_instruction_type_sem sr mr M F L [] (to_e_list es') ψ L.
   Admitted.
@@ -445,10 +435,8 @@ Section Fundamental.
   Lemma compat_ungroup M F L wl wl' es' τs κ :
     let me := me_of_context M mr in
     let fe := fe_of_context F in
-    local_ctx_ok F L ->
-    Forall (has_mono_rep F) τs ->
-    has_kind F (ProdT κ τs) κ ->
     let ψ := InstrT [ProdT κ τs] τs in
+    has_instruction_type_ok F ψ L ->
     run_codegen (compile_instr me fe (IUngroup ψ)) wl = inr ((), wl', es') ->
     ⊢ have_instruction_type_sem sr mr M F L [] (to_e_list es') ψ L.
   Admitted.
@@ -456,9 +444,9 @@ Section Fundamental.
   Lemma compat_fold M F L wl wl' es' τ κ :
     let me := me_of_context M mr in
     let fe := fe_of_context F in
-    has_kind F (RecT κ τ) κ ->
     let τ0 := subst_type VarM VarR VarS (unscoped.scons (RecT κ τ) VarT) τ in
     let ψ := InstrT [τ0] [RecT κ τ] in
+    has_instruction_type_ok F ψ L ->
     run_codegen (compile_instr me fe (IFold ψ)) wl = inr ((), wl', es') ->
     ⊢ have_instruction_type_sem sr mr M F L [] (to_e_list es') ψ L.
   Admitted.
@@ -468,6 +456,7 @@ Section Fundamental.
     let fe := fe_of_context F in
     let τ0 := subst_type VarM VarR VarS (unscoped.scons (RecT κ τ) VarT) τ in
     let ψ := InstrT [RecT κ τ] [τ0] in
+    has_instruction_type_ok F ψ L ->
     run_codegen (compile_instr me fe (IUnfold ψ)) wl = inr ((), wl', es') ->
     ⊢ have_instruction_type_sem sr mr M F L [] (to_e_list es') ψ L.
   Admitted.
@@ -475,46 +464,46 @@ Section Fundamental.
   Lemma compat_pack M F L wl wl' es' τ τ' :
     let me := me_of_context M mr in
     let fe := fe_of_context F in
-    packed_existential F τ τ' ->
     let ψ := InstrT [τ] [τ'] in
+    packed_existential F τ τ' ->
+    has_instruction_type_ok F ψ L ->
     run_codegen (compile_instr me fe (IPack ψ)) wl = inr ((), wl', es') ->
     ⊢ have_instruction_type_sem sr mr M F L [] (to_e_list es') ψ L.
   Admitted.
 
-  Lemma compat_unpack M F F0 L L' L0 L0' wl wl' es' es es0 ψ ψ0 :
+  Lemma compat_unpack M F F0 L L' L0 L0' wl wl' es es' es0 ψ ψ0 :
     let me := me_of_context M mr in
     let fe := fe_of_context F in
     unpacked_existential F L es ψ L' F0 L0 es0 ψ0 L0' ->
+    has_instruction_type_ok F ψ L' ->
     (forall wl wl' es',
-      let fe0 := fe_of_context F0 in
-      run_codegen (compile_instrs me fe0 es0) wl = inr ((), wl', es') ->
-      ⊢ have_instruction_type_sem sr mr M F0 L0 wl' (to_e_list es') ψ0 L0') ->
+        let fe0 := fe_of_context F0 in
+        run_codegen (compile_instrs me fe0 es0) wl = inr ((), wl', es') ->
+        ⊢ have_instruction_type_sem sr mr M F0 L0 wl' (to_e_list es') ψ0 L0') ->
     run_codegen (compile_instr me fe (IUnpack ψ L' es)) wl = inr ((), wl', es') ->
     ⊢ have_instruction_type_sem sr mr M F L [] (to_e_list es') ψ L'.
   Admitted.
 
-  Lemma compat_wrap M F L wl wl' es' τ0 ρ0 ρ ιs0 ιs χ δ :
+  Lemma compat_wrap M F L wl wl' es' τ0 ρ κ ιs ιs0 :
     let me := me_of_context M mr in
     let fe := fe_of_context F in
-    has_kind F τ0 (VALTYPE ρ0 χ δ) ->
-    eval_rep ρ0 = Some ιs0 ->
+    let ψ := InstrT [τ0] [RepT κ ρ τ0] in
+    type_rep_eval F τ0 ιs0 ->
     eval_rep ρ = Some ιs ->
     convertible_to ιs0 ιs ->
-    let τ := RepT (VALTYPE ρ χ δ) ρ τ0 in
-    let ψ := InstrT [τ0] [τ] in
+    has_instruction_type_ok F ψ L ->
     run_codegen (compile_instr me fe (IWrap ψ)) wl = inr ((), wl', es') ->
     ⊢ have_instruction_type_sem sr mr M F L [] (to_e_list es') ψ L.
   Admitted.
 
-  Lemma compat_unwrap M F L wl wl' es' τ0 ρ0 ρ ιs0 ιs χ δ :
+  Lemma compat_unwrap M F L wl wl' es' τ0 ρ κ ιs ιs0 :
     let me := me_of_context M mr in
     let fe := fe_of_context F in
-    has_kind F τ0 (VALTYPE ρ0 χ δ) ->
-    eval_rep ρ0 = Some ιs0 ->
+    let ψ := InstrT [RepT κ ρ τ0] [τ0] in
+    type_rep_eval F τ0 ιs0 ->
     eval_rep ρ = Some ιs ->
     convertible_to ιs0 ιs ->
-    let τ := RepT (VALTYPE ρ χ δ) ρ τ0 in
-    let ψ := InstrT [τ] [τ0] in
+    has_instruction_type_ok F ψ L ->
     run_codegen (compile_instr me fe (IUnwrap ψ)) wl = inr ((), wl', es') ->
     ⊢ have_instruction_type_sem sr mr M F L [] (to_e_list es') ψ L.
   Admitted.
@@ -523,6 +512,7 @@ Section Fundamental.
     let me := me_of_context M mr in
     let fe := fe_of_context F in
     let ψ := InstrT [type_i32] [type_i31] in
+    has_instruction_type_ok F ψ L ->
     run_codegen (compile_instr me fe (ITag ψ)) wl = inr ((), wl', es') ->
     ⊢ have_instruction_type_sem sr mr M F L [] (to_e_list es') ψ L.
   Admitted.
@@ -531,93 +521,85 @@ Section Fundamental.
     let me := me_of_context M mr in
     let fe := fe_of_context F in
     let ψ := InstrT [type_i31] [type_i32] in
+    has_instruction_type_ok F ψ L ->
     run_codegen (compile_instr me fe (IUntag ψ)) wl = inr ((), wl', es') ->
     ⊢ have_instruction_type_sem sr mr M F L [] (to_e_list es') ψ L.
   Admitted.
 
-  Lemma compat_ref_new M F L wl wl' es' μ τ τ' κ :
+  Lemma compat_ref_new M F L wl wl' es' τ τ' κ μ :
     let me := me_of_context M mr in
     let fe := fe_of_context F in
+    let ψ := InstrT [τ] [RefT κ μ τ'] in
     mono_mem μ ->
     stores_as F τ τ' ->
-    let τ_ref := RefT κ μ τ' in
-    has_kind F τ κ ->
-    let ψ := InstrT [τ] [τ_ref] in
+    has_instruction_type_ok F ψ L ->
     run_codegen (compile_instr me fe (IRefNew ψ)) wl = inr ((), wl', es') ->
     ⊢ have_instruction_type_sem sr mr M F L [] (to_e_list es') ψ L.
   Admitted.
 
-  Lemma compat_ref_load M F L wl wl' es' μ π τ τ_val pr ρ δ κ :
+  Lemma compat_ref_load M F L wl wl' es' π pr κ μ τ τval :
     let me := me_of_context M mr in
     let fe := fe_of_context F in
+    let ψ := InstrT [RefT κ μ τ] [RefT κ μ τ; τval] in
     resolve_path τ π None pr ->
+    has_copyability F pr.(pr_target) ImCopy ->
+    loads_as F pr.(pr_target) τval ->
     Forall (mono_size F) pr.(pr_prefix) ->
-    has_kind F pr.(pr_target) (VALTYPE ρ ImCopy δ) ->
-    loads_as F pr.(pr_target) τ_val ->
-    rep_ok kc_empty ρ ->
-    let τ_ref := RefT κ μ τ in
-    has_kind F τ_ref κ ->
-    let ψ := InstrT [τ_ref] [τ_ref; τ_val] in
+    has_instruction_type_ok F ψ L ->
     run_codegen (compile_instr me fe (IRefLoad ψ π)) wl = inr ((), wl', es') ->
     ⊢ have_instruction_type_sem sr mr M F L [] (to_e_list es') ψ L.
   Admitted.
 
-  Lemma compat_ref_store M F L wl wl' es' μ π τ τ_val pr κ :
+  Lemma compat_ref_store M F L wl wl' es' π pr κ μ τ τval :
     let me := me_of_context M mr in
     let fe := fe_of_context F in
+    let ψ := InstrT [RefT κ μ τ; τval] [τ] in
     resolve_path τ π None pr ->
-    Forall (mono_size F) pr.(pr_prefix) ->
     has_dropability F pr.(pr_target) ImDrop ->
-    stores_as F τ_val pr.(pr_target) ->
-    let τ_ref := RefT κ μ τ in
-    let ψ := InstrT [τ_ref; τ_val] [τ] in
-    run_codegen (compile_instr me fe (IRefStore ψ π)) wl = inr ((), wl', es') ->
-    ⊢ have_instruction_type_sem sr mr M F L [] (to_e_list es') ψ L.
-  Admitted.
-
-  Lemma compat_ref_mm_store M F L wl wl' es' π τ τ_val τ_val' pr κ κ' σ σ' δ :
-    let me := me_of_context M mr in
-    let fe := fe_of_context F in
-    resolve_path τ π (Some τ_val') pr ->
+    stores_as F τval pr.(pr_target) ->
     Forall (mono_size F) pr.(pr_prefix) ->
-    stores_as F τ_val τ_val' ->
-    has_kind F pr.(pr_target) (MEMTYPE (Sized σ) (ConstM MemMM) ImDrop) ->
-    has_kind F τ_val' (MEMTYPE (Sized σ') (ConstM MemMM) δ) ->
-    size_eq σ σ' ->
-    let τ_ref := RefT κ (ConstM MemMM) τ in
-    let τ_ref' := RefT κ' (ConstM MemMM) pr.(pr_replaced) in
-    has_kind F τ_ref κ ->
-    has_kind F τ_ref' κ' ->
-    let ψ := InstrT [τ_ref; τ_val] [τ_ref'] in
+    has_instruction_type_ok F ψ L ->
     run_codegen (compile_instr me fe (IRefStore ψ π)) wl = inr ((), wl', es') ->
     ⊢ have_instruction_type_sem sr mr M F L [] (to_e_list es') ψ L.
   Admitted.
 
-  Lemma compat_ref_swap M F L wl wl' es' π τ τ_val pr κ μ :
+  Lemma compat_ref_mm_store M F L wl wl' es' π pr κ κ' τ τval τmem :
     let me := me_of_context M mr in
     let fe := fe_of_context F in
+    let ψ := InstrT [RefT κ (ConstM MemMM) τ; τval] [RefT κ' (ConstM MemMM) pr.(pr_replaced)] in
+    stores_as F τval τmem ->
+    resolve_path τ π (Some τmem) pr ->
+    has_dropability F pr.(pr_target) ImDrop ->
+    type_size_eq F pr.(pr_target) τmem ->
+    Forall (mono_size F) pr.(pr_prefix) ->
+    has_instruction_type_ok F ψ L ->
+    run_codegen (compile_instr me fe (IRefStore ψ π)) wl = inr ((), wl', es') ->
+    ⊢ have_instruction_type_sem sr mr M F L [] (to_e_list es') ψ L.
+  Admitted.
+
+  Lemma compat_ref_swap M F L wl wl' es' π pr κ μ τ τval :
+    let me := me_of_context M mr in
+    let fe := fe_of_context F in
+    let ψ := InstrT [RefT κ μ τ; τval] [RefT κ μ τ; τval] in
     resolve_path τ π None pr ->
     Forall (mono_size F) pr.(pr_prefix) ->
-    loads_as F τ_val pr.(pr_target) ->
-    let τ_ref := RefT κ μ τ in
-    let ψ := InstrT [τ_ref; τ_val] [τ_ref; τ_val] in
+    loads_as F τval pr.(pr_target) ->
+    has_instruction_type_ok F ψ L ->
     run_codegen (compile_instr me fe (IRefSwap ψ π)) wl = inr ((), wl', es') ->
     ⊢ have_instruction_type_sem sr mr M F L [] (to_e_list es') ψ L.
   Admitted.
 
-  Lemma compat_ref_mm_swap M F L wl wl' es' π τ τ_val τ_val' τ__π κ κ' pr :
+  Lemma compat_ref_mm_swap M F L wl wl' es' π pr κ κ' τ τval τval' τmem :
     let me := me_of_context M mr in
     let fe := fe_of_context F in
-    resolve_path τ π (Some τ_val') pr ->
+    let ψ :=
+      InstrT [RefT κ (ConstM MemMM) τ; τval'] [RefT κ' (ConstM MemMM) pr.(pr_replaced); τval]
+    in
+    stores_as F τval τmem ->
+    resolve_path τ π (Some τmem) pr ->
     Forall (mono_size F) pr.(pr_prefix) ->
-    stores_as F τ_val τ_val' ->
-    loads_as F pr.(pr_target) τ__π ->
-    has_mono_rep F τ__π ->
-    let τ_ref := RefT κ (ConstM MemMM) τ in
-    let τ_ref' := RefT κ' (ConstM MemMM) pr.(pr_replaced) in
-    has_kind F τ_ref κ ->
-    has_kind F τ_ref' κ' ->
-    let ψ := InstrT [τ_ref; τ_val] [τ_ref'; τ__π] in
+    loads_as F pr.(pr_target) τval ->
+    has_instruction_type_ok F ψ L ->
     run_codegen (compile_instr me fe (IRefSwap ψ π)) wl = inr ((), wl', es') ->
     ⊢ have_instruction_type_sem sr mr M F L [] (to_e_list es') ψ L.
   Admitted.
@@ -710,7 +692,7 @@ Section Fundamental.
     - eapply compat_ref_store; eassumption.
     - eapply compat_ref_mm_store; eassumption.
     - eapply compat_ref_swap; eassumption.
-    - eapply compat_ref_mm_swap; eassumption.
+    - eapply compat_ref_mm_swap with (τmem := τmem); eassumption.
     - eapply compat_nil; eassumption.
     - eapply compat_cons; eassumption.
     - eapply compat_frame; eassumption.
